relational spec and attempt of a proof

c/poc/strlen_spec.v
@@ -55,10 +55,6 @@ Definition strlen_C_correct := forall m p z m' bs, strlen_C_byte m p = Some (z,m
 
 (** Low-level specification *)
 
-Inductive strlen_spec_C : mem -> addr -> option (Z*mem) -> Prop :=
-| UninitMemory : forall m addr, not (Mem.valid_block m (block_of addr)) -> strlen_spec_C m addr None. (* Block of addr is not initialized in m *)
-(*TODO *)
-
 (* true if the integer value read is zero - end of string *)
 Definition is_null (v : Values.val) :=
   match v with
@@ -66,12 +62,11 @@ Definition is_null (v : Values.val) :=
   | _ => false
   end.
 
-Definition chunk : memory_chunk := Mint8signed. (* not quite sure how to deal with the memory chunks *)
+Definition chunk : memory_chunk := Mint8signed. (* that's what we read from memory *)
 Definition INTSIZE := (nat_of_Z Int.modulus).
 
 
-Definition strlen_C (m : mem) (b: block) (ofs : Z) := 
-  let fix strlen_fun_C (m : mem) (b : block) (ofs : Z) (l: Z) (intrange : nat) {struct intrange} : option (Z*mem):=
+Fixpoint strlen_fun_C (m : mem) (b : block) (ofs : Z) (l: Z) (intrange : nat) {struct intrange} : option (Z*mem):= (* maybe nat output? *)
       match intrange with
       | O => None (* out of int range *)
       | S n => match valid_block_b m b, Mem.load chunk m b ofs with (* checking if b is a valid reference in m, loading value from memory *)
@@ -80,10 +75,44 @@ Definition strlen_C (m : mem) (b: block) (ofs : Z) :=
                 then Some (l, m) else strlen_fun_C m b (ofs + 1) (l + 1) n  
               | _, _ => None (* address not readable or b not allocates *)
               end
-      end
-  in strlen_fun_C m b ofs 0 INTSIZE.
+      end.
+
+Definition strlen_C_fun_spec (m : mem) (b: block) (ofs : Z) :=  strlen_fun_C m b ofs 0 INTSIZE.
 
 
+(* Relational spec, to use in the proofs *)
+
+Inductive strlen_C_rel_spec : Mem.mem -> block -> Z -> option (nat * mem)-> Prop
+  := | CorrectRun :  forall n m b ofs,
+    (n < INTSIZE)%nat ->
+    forall v, (* Mem.valid_block m b -> *) (* ignore for now *)
+              Mem.load chunk m b ofs = Some v ->
+              (exists z, v = Vint z) -> (* not Undef *)
+              Mem.load chunk m b (ofs + (Z_of_nat n)) = Some (Vint (Int.repr 0)) ->
+              strlen_C_rel_spec m b ofs (Some (n,m))
+  | OutOfRange :   forall n m b ofs,
+    (n > INTSIZE)%nat ->
+    forall v, (* Mem.valid_block m b -> *)
+              Mem.load chunk m b ofs = Some v ->
+              Mem.load chunk m b (ofs + (Z_of_nat n)) = Some (Vint (Int.repr 0)) ->
+              strlen_C_rel_spec m b ofs None
+
+
+  | MemoryLoadZero :  forall n m b ofs,
+    (n < INTSIZE)%nat ->
+              (* Mem.valid_block m b -> *)
+              Mem.load chunk m b ofs = None ->
+              strlen_C_rel_spec m b ofs None
+
+  | MemoryLoadSucc : forall n m b ofs,
+       (n < INTSIZE)%nat ->
+      forall v, (* Mem.valid_block m b -> *)
+              Mem.load chunk m b ofs = Some v ->
+              Mem.load chunk m b (ofs + (Z_of_nat n)) = Some (Vint (Int.repr 0)) ->
+              (exists n', (n' < n)%nat /\ Mem.load chunk m b (ofs + (Z_of_nat n')) = None) ->
+              strlen_C_rel_spec m b ofs None.
+                                                                           
+                            
 (* Semantics of a C light function: *)
 
 (* strlen C light AST *)
@@ -123,12 +152,13 @@ Definition ge := globalenv prog. *)
 
 Parameter ge : genv. (* global environment, maps id to block, pointers to definitions of functions *)
 Definition bigStepExec := ClightBigstep.exec_stmt. (* evaluation of statements*)
-Definition t := ((E0**E0)**E0). (* trace, E0 is an empty trace *)
+Definition t := ((E0**E0)**E0). (* trace of this particular program, E0 is an empty trace *)
 
-(* One direction of correctness, for now the statement seems wrong *)
-Definition strlen_C_exec_corr :
+(* One direction of correctness, using functional spec, below relational with proof attempt *)
+
+ Definition strlen_C_fun_corr_r :
   forall (m : Mem.mem) (b : block) (ofs : Z) (e : env) (le : temp_env) (z : Z),
-    strlen_C m b ofs = Some (z,m) ->
+    strlen_C_fun_spec m b ofs = Some (z,m) ->
     le!_s = Some (Vptr b (Ptrofs.repr ofs)) -> (* input parameter _s assigned value of address (b,ofs) in le *)
     exists le', le'!_i = Some (Vint (Int.repr z)) /\ (* output _i assigned value z in le *)
                 bigStepExec ge e le m f_strlen.(fn_body) t le' m (Out_return (Some (Vint (Int.repr z),tuint))).
@@ -138,17 +168,132 @@ Proof.
   exists (Maps.PTree.set _i (Vint (Int.repr z)) le).
   split.
   - apply Maps.PTree.gss.
-  - repeat econstructor.
+    - repeat econstructor.
     + rewrite PTree.gso. apply H0. eapply Pos.succ_discr. 
     + apply PTree.gss.
-    + repeat econstructor. 
-    + simpl. (* rewrite <- (ptr_ofs_eq ofs) - arithmetic on ptrofs. now need assumptions on memory, get from a lemma about strlen *) admit.
+    + repeat econstructor.
+    + simpl. admit.
     + simpl.  admit.
     + simpl. admit.
     + simpl.  admit.
-      Admitted.
+Admitted.
 
-(* Examples of running a program: to see what assumptions need in the proof *)
+ (* Find proofs on arithmetic on ptrofs type to rewrite this *)
+      Hypothesis ptr_ofs_eq : forall ofs, ofs = (Ptrofs.unsigned
+       (Ptrofs.add (Ptrofs.repr ofs)
+                   (Ptrofs.mul (Ptrofs.repr 1) (Ptrofs.of_intu (Int.repr 0))))). 
+
+Definition strlen_C_rel_corr_r : forall n m b ofs e le,
+    strlen_C_rel_spec m b ofs (Some (n,m)) ->
+    le!_s = Some (Vptr b (Ptrofs.repr ofs)) -> 
+    exists le', le'!_i = Some (Vint (Int.repr (Z_of_nat n))) /\ 
+           bigStepExec ge e le m f_strlen.(fn_body) t le' m (Out_return (Some (Vint (Int.repr (Z_of_nat n)),tuint))).
+Proof.
+  induction n.
+  (* Base case. *)
+  intros.
+  inversion H. unfold chunk in *. destruct H4.
+  exists (Maps.PTree.set _i (Vint (Int.repr (Z.of_nat 0))) le).
+  split.
+  - apply Maps.PTree.gss.
+  - repeat econstructor.
+    + rewrite PTree.gso. apply H0. eapply Pos.succ_discr. 
+    + apply PTree.gss.
+    + repeat econstructor.
+    + simpl. rewrite <- ptr_ofs_eq. apply H3.
+    + cbn. rewrite -> H4. reflexivity.
+    + cbn. unfold Val.of_bool. simpl in H8. rewrite H4 in H3.  rewrite Z.add_0_r in H8.  rewrite H8 in H3. inversion H3. reflexivity.
+    + Hypothesis fls : negb (Int.eq Int.zero Int.zero) = false.
+      rewrite fls. econstructor.
+    + apply PTree.gss.
+Admitted.
+
+(* Tactic for inversion  *)
+
+ Ltac invertSem :=
+        match goal with
+          | [H : context[exec_stmt] |- _] =>
+            inversion H ; clear H 
+          | [H : context[eval_expr] |- _] =>
+            inversion H ; clear H
+          | [H : context[eval_lvalue] |- _] =>
+            inversion H ; clear H 
+          | [H : context[bool_val] |- _] =>
+            inversion H ; clear H
+          | [H : context[deref_loc] |- _] =>
+            inversion H ; clear H  
+          | [H : context[sem_binary_operation] |- _] =>
+            inversion H ; clear H  
+          | [H : context[access_mode] |- _] =>
+            inversion H ; clear H  
+          | _ => idtac
+        end.    
+
+
+ Ltac solve_by_inverts n :=
+   match n with
+   | O => idtac
+   | S (?n') => invertSem ; subst ; solve_by_inverts n'
+   end.
+
+ (* behaves differently than the above: 
+
+  Ltac invert_clear :=
+        match goal with
+          | [H : context[exec_stmt] |- _] =>
+            inversion_clear H 
+          | [H : context[eval_expr] |- _] =>
+            inversion_clear H 
+          | [H : context[eval_lvalue] |- _] =>
+            inversion_clear H 
+          | [H : context[bool_val] |- _] =>
+            inversion_clear H  
+          | [H : context[deref_loc] |- _] =>
+            inversion_clear H  
+          | [H : context[sem_binary_operation] |- _] =>
+           inversion_clear H  
+          | [H : context[access_mode] |- _] =>
+            inversion_clear H  
+          | _ => idtac
+        end.    
+
+
+ Ltac solve_by_inverts n :=
+   match n with
+   | O => subst
+   | S (?n') =>  invert_clear; solve_by_inverts n'
+   end.
+
+  *)
+ 
+ Definition strlen_C_rel_corr_l : forall n m b ofs e le,
+     (n < INTSIZE)%nat ->
+     le!_s = Some (Vptr b (Ptrofs.repr ofs)) ->
+     (exists le', le'!_i = Some (Vint (Int.repr (Z_of_nat n))) /\ 
+                bigStepExec ge e le m f_strlen.(fn_body) t le' m (Out_return (Some (Vint (Int.repr (Z_of_nat n)),tuint))))
+           -> strlen_C_spec m b ofs (Some (n,m)).
+Proof.
+  intros.
+  repeat destruct H1.
+  inversion H2.
+  solve_by_inverts 5%nat. solve_by_inverts 15%nat. (* TODO: fix the tactic *)  Admitted.
+
+
+Definition strlen_C_exec_corr_l :
+  forall (m : Mem.mem) (b : block) (ofs : Z) (e : env) (le : temp_env) (z : Z),
+    le!_s = Some (Vptr b (Ptrofs.repr ofs)) -> 
+    (exists le', le'!_i = Some (Vint (Int.repr z)) /\ 
+                bigStepExec ge e le m f_strlen.(fn_body) t le' m (Out_return (Some (Vint (Int.repr z),tuint))))
+           -> strlen_C m b ofs = Some (z,m).
+Proof.
+  intros.
+  repeat destruct H0.
+  inversion H1.
+  solve_by_inverts 5%nat. solve_by_inverts 15%nat. 
+  unfold strlen_C.  unfold strlen_fun_C. unfold Mem.loadv in H9.
+  Admitted.
+              
+(* Examples of running a program: to see what assumptions need in the proof, experiments *)
 
 Parameter hi : Z.
 Definition init_mem := fst (Mem.alloc Mem.empty 0 hi).
@@ -161,10 +306,7 @@ Hypothesis ofs_le_hi : ofs' < hi.
 Definition init_mem1 := 
   Mem.store Mint8signed init_mem b' ofs' (Vint (Int.repr 0)).
 
-(* Find proofs on arithmetic on ptrofs type *)
-Hypothesis ptr_ofs_eq : forall ofs, ofs = (Ptrofs.unsigned
-       (Ptrofs.add (Ptrofs.repr ofs)
-                   (Ptrofs.mul (Ptrofs.repr 1) (Ptrofs.of_intu (Int.repr 0))))).
+
 
 Lemma example_comp : forall m le e, init_mem1 = Some m ->
                              le!_s = Some (Vptr b' (Ptrofs.repr ofs')) ->
